Instance/Lambda/Exp.v
@@ -24,22 +24,22 @@ Derive Signature NoConfusion EqDec for Var.
 Inductive Exp Γ : Ty → Type :=
   | EUnit               : Exp Γ TyUnit
 
-  (* | Pair {τ1 τ2}        : Exp Γ τ1 → Exp Γ τ2 → Exp Γ (TyPair τ1 τ2) *)
-  (* | Fst {τ1 τ2}         : Exp Γ (TyPair τ1 τ2) → Exp Γ τ1 *)
-  (* | Snd {τ1 τ2}         : Exp Γ (TyPair τ1 τ2) → Exp Γ τ2 *)
+  | Pair {τ1 τ2}        : Exp Γ τ1 → Exp Γ τ2 → Exp Γ (TyPair τ1 τ2)
+  | Fst {τ1 τ2}         : Exp Γ (TyPair τ1 τ2) → Exp Γ τ1
+  | Snd {τ1 τ2}         : Exp Γ (TyPair τ1 τ2) → Exp Γ τ2
 
   | VAR {τ}             : Var Γ τ → Exp Γ τ
   | LAM {dom cod}       : Exp (dom :: Γ) cod → Exp Γ (dom ⟶ cod)
   | APP {dom cod}       : Exp Γ (dom ⟶ cod) → Exp Γ dom → Exp Γ cod.
 
-Derive Signature NoConfusionHom EqDec for Exp.
+Derive Signature NoConfusionHom Subterm EqDec for Exp.
 
 Fixpoint Exp_size {Γ τ} (e : Exp Γ τ) : nat :=
   match e with
   | EUnit _       => 1
-  (* | Pair _ x y    => 1 + Exp_size x + Exp_size y *)
-  (* | Fst _ p       => 1 + Exp_size p *)
-  (* | Snd _ p       => 1 + Exp_size p *)
+  | Pair _ x y    => 1 + Exp_size x + Exp_size y
+  | Fst _ p       => 1 + Exp_size p
+  | Snd _ p       => 1 + Exp_size p
   | VAR _ v       => 1
   | LAM _ e       => 1 + Exp_size e
   | APP _ e1 e2   => 1 + Exp_size e1 + Exp_size e2
@@ -52,9 +52,9 @@ Proof. repeat intro; subst; contradiction. Qed.
 End Exp.
 
 Arguments EUnit {Γ}.
-(* Arguments Pair {Γ τ1 τ2} _ _. *)
-(* Arguments Fst {Γ τ1 τ2} _. *)
-(* Arguments Snd {Γ τ1 τ2} _. *)
+Arguments Pair {Γ τ1 τ2} _ _.
+Arguments Fst {Γ τ1 τ2} _.
+Arguments Snd {Γ τ1 τ2} _.
 Arguments VAR {Γ τ} _.
 Arguments LAM {Γ dom cod} _.
 Arguments APP {Γ dom cod} _ _.
