Instance/Lambda/Full.v
@@ -25,16 +25,20 @@ Open Scope Ty_scope.
 (* A context defines a hole which, after substitution, yields an expression of
    the index type. *)
 Inductive Frame Γ : Ty → Ty → Type :=
+  | F_PairL {τ1 τ2}  : Exp Γ τ2 → Frame Γ τ1 (τ1 × τ2)
+  | F_PairR {τ1 τ2}  : Exp Γ τ1 → Frame Γ τ2 (τ1 × τ2)
+  | F_Fst {τ1 τ2}    : Frame Γ (τ1 × τ2) τ1
+  | F_Snd {τ1 τ2}    : Frame Γ (τ1 × τ2) τ2
   | F_AppL {dom cod} : Exp Γ dom → Frame Γ (dom ⟶ cod) cod
   | F_AppR {dom cod} : Exp Γ (dom ⟶ cod) → Frame Γ dom cod.
 
-Derive Signature NoConfusion NoConfusionHom Subterm EqDec for Frame.
+Derive Signature NoConfusion Subterm for Frame.
 
 Inductive Ctxt Γ : Ty → Ty → Type :=
   | C_Nil {τ}         : Ctxt Γ τ τ
   | C_Cons {τ τ' τ''} : Frame Γ τ' τ → Ctxt Γ τ'' τ' → Ctxt Γ τ'' τ.
 
-Derive Signature NoConfusion NoConfusionHom Subterm EqDec for Ctxt.
+Derive Signature NoConfusion NoConfusionHom Subterm for Ctxt.
 
 (* [Ctxt] forms a category with objects = types and morphisms = contexts. *)
 
@@ -64,7 +68,15 @@ Proof. induction C; simpl; auto; now f_equal. Qed.
 Inductive Redex {Γ} : ∀ {τ}, Exp Γ τ → Exp Γ τ → Prop :=
   | R_Beta {dom cod} (e : Exp (dom :: Γ) cod) v :
     ValueP v →
-    Redex (APP (LAM e) v) (SubExp {|| v ||} e).
+    Redex (APP (LAM e) v) (SubExp {|| v ||} e)
+  | R_Fst {τ1 τ2} (x : Exp Γ τ1) (y : Exp Γ τ2) :
+    ValueP x →
+    ValueP y →
+    Redex (Fst (Pair x y)) x
+  | R_Snd {τ1 τ2} (x : Exp Γ τ1) (y : Exp Γ τ2) :
+    ValueP x →
+    ValueP y →
+    Redex (Snd (Pair x y)) y.
 
 Derive Signature for Redex.
 
@@ -72,6 +84,23 @@ Unset Elimination Schemes.
 
 Inductive Plug {Γ τ'} (e : Exp Γ τ') : ∀ {τ}, Ctxt Γ τ' τ → Exp Γ τ → Prop :=
   | Plug_Hole : Plug e (C_Nil _) e
+
+  | Plug_PairL {τ1 τ2} {C : Ctxt Γ τ' τ1} {e' : Exp Γ τ1} {e2 : Exp Γ τ2} :
+    Plug e C e' →
+    Plug e (C_Cons _ (F_PairL _ e2) C) (Pair e' e2)
+
+  | Plug_PairR {τ1 τ2} {C : Ctxt Γ τ' τ2} {e1 : Exp Γ τ1} {e' : Exp Γ τ2} :
+    ValueP e1 →
+    Plug e C e' →
+    Plug e (C_Cons _ (F_PairR _ e1) C) (Pair e1 e')
+
+  | Plug_Fst {τ1 τ2} {C : Ctxt Γ τ' (τ1 × τ2)} {e' : Exp Γ (τ1 × τ2)} :
+    Plug e C e' →
+    Plug e (C_Cons _ (F_Fst _) C) (Fst e')
+
+  | Plug_Snd {τ1 τ2} {C : Ctxt Γ τ' (τ1 × τ2)} {e' : Exp Γ (τ1 × τ2)} :
+    Plug e C e' →
+    Plug e (C_Cons _ (F_Snd _) C) (Snd e')
 
   | Plug_AppL {dom cod} {C : Ctxt Γ τ' (dom ⟶ cod)}
               {e' : Exp Γ (dom ⟶ cod)} {e2 : Exp Γ dom} :
@@ -102,18 +131,21 @@ Fixpoint Plug_comp {Γ τ τ' τ''}
          (P : Plug x C' y) (P' : Plug y C z) :
   Plug x (Ctxt_comp C C') z :=
   match P' with
-  | Plug_Hole _      => P
-  | Plug_AppL _ p'   => Plug_AppL _ (Plug_comp P p')
-  | Plug_AppR _ V p' => Plug_AppR _ V (Plug_comp P p')
+  | Plug_Hole _       => P
+  | Plug_PairL _ p'   => Plug_PairL _ (Plug_comp P p')
+  | Plug_PairR _ V p' => Plug_PairR _ V (Plug_comp P p')
+  | Plug_Fst _ p'     => Plug_Fst _ (Plug_comp P p')
+  | Plug_Snd _ p'     => Plug_Snd _ (Plug_comp P p')
+  | Plug_AppL _ p'    => Plug_AppL _ (Plug_comp P p')
+  | Plug_AppR _ V p'  => Plug_AppR _ V (Plug_comp P p')
   end.
 
+(*
 (* This should be provable, but the dependent types get in the way. *)
 Theorem Plug_id_left {Γ τ τ'} {C : Ctxt Γ τ' τ} {x : Exp Γ τ'} {y : Exp Γ τ}
         (P : Plug x C y) :
   Plug_comp Plug_id P ~= P.
-Proof.
-  dependent induction P; simpl in *; auto.
-Abort.
+*)
 
 Reserved Notation " t '--->' t' " (at level 40).
 
@@ -137,6 +169,19 @@ Theorem strong_progress {τ} (e : Exp [] τ) :
 Proof.
   dependent induction e; reduce.
   - now left; constructor.
+  - destruct IHe1 as [V1|[e1' H1']];
+    destruct IHe2 as [V2|[e2' H2']].
+    + now left; constructor.
+    + dependent elimination H2'; now eauto 6.
+    + dependent elimination H1'; now eauto 6.
+    + dependent elimination H1';
+      dependent elimination H2'; now eauto 6.
+  - destruct IHe as [V|[e' H']].
+    + dependent elimination V;  now eauto 6.
+    + dependent elimination H'; now eauto 6.
+  - destruct IHe as [V|[e' H']].
+    + dependent elimination V;  now eauto 6.
+    + dependent elimination H'; now eauto 6.
   - now inv v.
   - now left; constructor.
   - right.
@@ -148,80 +193,14 @@ Proof.
     + dependent elimination H1'; now eauto 6.
 Qed.
 
-Lemma Plug_value {Γ τ} {C : Ctxt Γ τ τ} (e v : Exp Γ τ) :
-  ValueP v → Plug e C v → C = C_Nil _ ∧ e = v.
-Proof.
-  intros.
-  dependent elimination H0;
-  now inv H.
-Qed.
-
-Lemma Value_not_redex {Γ τ} (e v : Exp Γ τ) :
-  ValueP v → ¬ Redex v e.
-Proof.
-  repeat intro.
-  dependent elimination H0;
-  now inv H.
-Qed.
-
-Lemma Value_cannot_start {Γ τ} {e e' : Exp Γ τ} :
-  (e ---> e') → ¬ ValueP e.
-Proof.
-  repeat intro.
-  dependent elimination H0;
-  inv H; inv H0; inv H2.
-Qed.
-
-Corollary Value_irreducible {Γ τ} {e e' : Exp Γ τ} :
-  ValueP e → ¬ (e ---> e').
-Proof.
-  repeat intro.
-  apply Value_cannot_start in H0.
-  contradiction.
-Qed.
-
+(*
 Lemma Plug_deterministic {Γ τ} e2 :
   ∀ τ' (C : Ctxt Γ τ' τ) e1 e1',
     Redex e1 e1' → Plug e1 C e2 →
   ∀ τ'' (C' : Ctxt Γ τ'' τ) f1 f1',
     Redex f1 f1' → Plug f1 C' e2 →
     τ' = τ'' ∧ C ~= C' ∧ e1 ~= f1.
-Proof.
-  intros τ' C e1 e1' R1 P1 τ'' C' f1 f1' R2 P2.
-  generalize dependent C'.
-  induction P1; intros; subst.
-  inv P2; auto.
-  - exfalso.
-    dependent elimination R1.
-    dependent elimination R2.
-    now inv H2.
-  - exfalso.
-    dependent elimination R1.
-    dependent elimination R2.
-    now inv H3.
-  - dependent elimination P2.
-    + exfalso.
-      dependent elimination R1.
-      dependent elimination R2.
-      now inv P1.
-    + intuition.
-      now destruct (IHP1 _ p); reduce.
-    + exfalso.
-      dependent elimination R1.
-      dependent elimination R2.
-      now inv P1.
-  - dependent elimination P2.
-    + exfalso.
-      dependent elimination R1.
-      dependent elimination R2.
-      now inv P1.
-    + exfalso.
-      dependent elimination R1.
-      dependent elimination R2.
-      now inv p.
-    + intuition.
-      now destruct (IHP1 _ p0); reduce.
-Qed.
+*)
 
 Lemma Plug_functional {Γ τ τ'} {C : Ctxt Γ τ' τ} e :
   ∀ e1, Plug e C e1 → ∀ e2, Plug e C e2 → e1 = e2.
@@ -229,6 +208,14 @@ Proof.
   intros.
   dependent induction H0.
   - now inv H.
+  - dependent destruction H.
+    now f_equal; auto.
+  - dependent destruction H.
+    now f_equal; auto.
+  - dependent destruction H.
+    now f_equal; auto.
+  - dependent destruction H.
+    now f_equal; auto.
   - dependent destruction H.
     now f_equal; auto.
   - dependent destruction H.
@@ -245,15 +232,22 @@ Proof.
     now f_equal; auto.
   - dependent destruction H.
     now f_equal; auto.
+  - dependent destruction H.
+    now f_equal; auto.
+  - dependent destruction H.
+    now f_equal; auto.
+  - dependent destruction H.
+    now f_equal; auto.
+  - dependent destruction H.
+    now f_equal; auto.
 Qed.
 
 Lemma Redex_deterministic {Γ τ} {e : Exp Γ τ} :
   ∀ e', Redex e e' → ∀ e'', Redex e e'' → e' = e''.
 Proof.
   intros.
-  dependent elimination H0.
-  dependent elimination H.
-  reflexivity.
+  dependent induction H0;
+  dependent elimination H; eauto.
 Qed.
 
 Lemma AppL_LAM {Γ dom cod} {e e' : Exp Γ (dom ⟶ cod)} {x : Exp Γ dom} :
@@ -278,16 +272,10 @@ Definition normal_form `(R : relation X) (t : X) : Prop :=
 Definition deterministic `(R : relation X) : Prop :=
   ∀ x y1 y2 : X, R x y1 → R x y2 → y1 = y2.
 
+(*
 Lemma value_is_nf {Γ τ} (v : Exp Γ τ) :
   ValueP v → normal_form Step v.
-Proof.
-  repeat intro.
-  dependent elimination H0.
-  dependent induction H.
-  dependent elimination p.
-  - now dependent elimination r.
-  - now dependent elimination p.
-Qed.
+*)
 
 End Full.
 
